Clap/eDSLState/Varstore.lean
@@ -1,5 +1,6 @@
 import Mathlib.Data.ZMod.Basic
 import Std.Data.ExtTreeMap
+import Clap.eDSLState.Wheels
 
 namespace Clap
 
@@ -7,20 +8,22 @@ abbrev VarStore (p : ℕ) := Std.ExtTreeMap ℕ (ZMod p) (cmp := compare)
 
 namespace VarStore
 
+variable {p : ℕ}
+
 @[grind =]
-instance {p : ℕ} : HasSubset (VarStore p) where
+instance : HasSubset (VarStore p) where
   Subset Γ1 Γ2 := ∀ k : ℕ, Γ1[k]?.isSome → Γ1[k]? = Γ2[k]?
 
-lemma hasSubset_def {p} {Γ₁ Γ₂ : VarStore p} :
+lemma hasSubset_def {Γ₁ Γ₂ : VarStore p} :
   (Γ₁ ⊆ Γ₂) = ∀ k : ℕ, Γ₁[k]?.isSome → Γ₁[k]? = Γ₂[k]? := rfl
 
-lemma subset_insert {p} {Γ : VarStore p} {k} {v} {h : k ∉ Γ}:
+lemma subset_insert {Γ : VarStore p} {k} {v} {h : k ∉ Γ}:
   Γ ⊆ Γ.insert k v
 := by
   aesop (add simp hasSubset_def) (add safe (by grind))
 
 @[grind _=_]
-lemma mem_iff_mem_keys {p} {Γ : VarStore p} {k}:
+lemma mem_iff_mem_keys {Γ : VarStore p} {k}:
   k ∈ Γ ↔ k ∈ Γ.keys
 := by
   grind
